open import Algebra.FunctionProperties
open import C.Base
open import C.Properties.Musical
open import C.Properties.State
open import Codata.Musical.Notation
open import Codata.Musical.Colist as Colist
open import Data.Bool as ğ”¹ using () renaming (Bool to ğ”¹)
open import Data.Empty
open import Data.Integer as â„¤ using (+_)
open import Data.Integer.Properties as â„¤â‚š using ()
open import Data.Nat as â„• using (â„•)
open import Data.Product using (âˆƒ ; _,_ ; âˆƒ-syntax ; projâ‚ ; projâ‚‚)
open import Data.Sum
open import Data.Vec
open import Function.Nary.NonDependent
open import Relation.Binary
open import Relation.Binary.PropositionalEquality
open import Relation.Nullary
open import Size

import Level
import Codata.Musical.Conat as Coâ„•

module C.Properties.Properties â¦ƒ _ : C â¦„ â¦ƒ _ : Semantics â¦„ where

open C â¦ƒ ... â¦„
open Semantics â¦ƒ ... â¦„
open â‰¡-Reasoning


-- EXPRESSION EQUIVALENCE

+-left-id : LeftIdentity _â‰…â‚‘_ (âŸª + 0 âŸ«) _+_
+-left-id e {E} {v} {w} 0+eâ‡’v eâ‡’w =
  let 0+eâ‡’0+w = +-eval (nat (+ 0)) eâ‡’w in
  let vâ‰¡0+w = âŠ¢-det 0+eâ‡’v 0+eâ‡’0+w in
  begin
    v
    â‰¡âŸ¨ vâ‰¡0+w âŸ©
    + 0 â„¤.+ w
    â‰¡âŸ¨ â„¤â‚š.+-identityË¡ w âŸ©
    w
  âˆ

+-right-id : RightIdentity _â‰…â‚‘_ (âŸª + 0 âŸ«) _+_
+-right-id e {E} {v} {w} e+0â‡’v eâ‡’w =
  let e+0â‡’w+0 = +-eval eâ‡’w (nat (+ 0)) in
  let vâ‰¡w+0 = âŠ¢-det e+0â‡’v e+0â‡’w+0 in
  begin
    v
    â‰¡âŸ¨ vâ‰¡w+0 âŸ©
    w â„¤.+ + 0
    â‰¡âŸ¨ â„¤â‚š.+-identityÊ³ w âŸ©
    w
  âˆ

+-id : Identity _â‰…â‚‘_ (âŸª + 0 âŸ«) _+_
+-id = +-left-id , +-right-id

+-assoc : Associative _â‰…â‚‘_ _+_
+-assoc x y z {E} {v} {w} [x+y]+zâ‡’v x+[y+z]â‡’w =
  let x' , â‡’x' = âŠ¢-total {e = x} in
  let y' , â‡’y' = âŠ¢-total {e = y} in
  let z' , â‡’z' = âŠ¢-total {e = z} in
  begin
    v
    â‰¡âŸ¨ âŠ¢-det [x+y]+zâ‡’v (+-eval (+-eval â‡’x' â‡’y') â‡’z') âŸ©
    (x' â„¤.+ y') â„¤.+ z'
    â‰¡âŸ¨ â„¤â‚š.+-assoc x' y' z' âŸ©
    x' â„¤.+ (y' â„¤.+ z')
    â‰¡âŸ¨ âŠ¢-det (+-eval â‡’x' (+-eval â‡’y' â‡’z')) x+[y+z]â‡’w âŸ©
    w
  âˆ

+-comm : Commutative _â‰…â‚‘_ _+_
+-comm x y {E} {v} {w} x+yâ‡’v y+xâ‡’w =
  let x' , â‡’x' = âŠ¢-total {e = x} in
  let y' , â‡’y' = âŠ¢-total {e = y} in
  begin
    v
    â‰¡âŸ¨ âŠ¢-det x+yâ‡’v (+-eval â‡’x' â‡’y') âŸ©
    x' â„¤.+ y'
    â‰¡âŸ¨ â„¤â‚š.+-comm x' y' âŸ©
    y' â„¤.+ x'
    â‰¡âŸ¨ âŠ¢-det (+-eval â‡’y' â‡’x') y+xâ‡’w âŸ©
    w
  âˆ

-- *-id : Identity _â‰…â‚‘_ (âŸ¨ + 1 âŸ©) _*_
-- *-zero : Zero _â‰…â‚‘_ (âŸ¨ + 0 âŸ©) _*_
-- *-assoc : Associative _â‰…â‚‘_ _*_
-- *-commute : Commutative _â‰…â‚‘_ _*_
-- âˆ¸-id : Identity _â‰…â‚‘_ (âŸ¨ + 0 âŸ©) _-_
-- /-id : Identity _â‰…â‚‘_ (âŸ¨ + 1 âŸ©) _/_
-- -- TODO: algebra properties of _<_ _<=_ _>_ _>=_ _==_ using standard library algebra
-- <-trans : âˆ€ { x y z : Expr Int } â†’ x < y â‰…â‚‘ true â†’ y < z â‰…â‚‘ true â†’ x < z â‰…â‚‘ true
-- ||-id : Identity _â‰…â‚‘_ false _||_
-- ||-zero : Zero _â‰…â‚‘_ true _||_
-- ||-assoc : Associative _â‰…â‚‘_ _||_
-- ||-commute : Commutative _â‰…â‚‘_ _||_
-- &&-id : Identity _â‰…â‚‘_ true _&&_
-- &&-zero : Zero _â‰…â‚‘_ false _&&_
-- &&-assoc : Associative _â‰…â‚‘_ _&&_
-- &&-commute : Commutative _â‰…â‚‘_ _&&_ 


-- PROGRAM EQUIVALENCE

L0 : âˆ€ { n } â†’ Levels n
L0 {0} = _
L0 {â„•.suc n} = Level.zero , L0

infix 0 _â‰…â‚š_
_â‰…â‚š_ : âˆ€ { n } { v : Sets n L0 } â†’ Rel (v â‡‰ Statement) Level.zero
_â‰…â‚š_ {0} x y = âˆ€ { k E } â†’ ğ’® x k E â‰…â‚› ğ’® y k E
_â‰…â‚š_ {â„•.suc n} {_ , v} x y = âˆ€ { r } â†’ _â‰…â‚š_ (x r) (y r)

â‰…â‚š-refl : âˆ€ { n } { v : Sets n L0 } â†’ Reflexive (_â‰…â‚š_ {v = v})
â‰…â‚š-refl {â„•.zero} {Level.lift _} {_} = â‰…â‚›-refl
â‰…â‚š-refl {â„•.suc n} {x , v} = (â‰…â‚š-refl {v = v})

â‰…â‚š-sym : âˆ€ { n } { v : Sets n L0 } â†’ Symmetric (_â‰…â‚š_ {v = v})
â‰…â‚š-sym {0} {lift} i~j = â‰…â‚›-sym i~j
â‰…â‚š-sym {â„•.suc n} {x , v} i~j = â‰…â‚š-sym {v = v} i~j

â‰…â‚š-trans : âˆ€ { n } { v : Sets n L0 } â†’ Transitive (_â‰…â‚š_ {v = v})
â‰…â‚š-trans {0} {lift} i~j j~k = â‰…â‚›-trans i~j j~k
â‰…â‚š-trans {â„•.suc n} {x , v} i~j j~k = â‰…â‚š-trans {v = v} i~j j~k

â‰…â‚š-equiv : âˆ€ { n } { v : Sets n L0 } â†’ IsEquivalence (_â‰…â‚š_ {v = v})
â‰…â‚š-equiv = record { refl = â‰…â‚š-refl ; sym = â‰…â‚š-sym ; trans = â‰…â‚š-trans }

â‰…â‚š-setoid : âˆ€ { n } { v : Sets n L0 } â†’ Setoid _ _
â‰…â‚š-setoid {i} {v = v} = record {
  Carrier = v â‡‰ Statement ;
  _â‰ˆ_ = _â‰…â‚š_ ;
  isEquivalence = â‰…â‚š-equiv }

import Relation.Binary.Reasoning.Setoid as Reasoning
module â‰…R = Reasoning (â‰…â‚š-setoid {0})
  renaming (_â‰ˆâŸ¨_âŸ©_ to _â‰…âŸ¨_âŸ©_ ; _â‰ˆË˜âŸ¨_âŸ©_ to _â‰…Ë˜âŸ¨_âŸ©_)
open â‰…R
module â‰ˆR = â‰ˆ-Reasoning
open â‰ˆR

postulate â‰…â‚š-cong : âˆ€ { n } { v : Sets n L0 } (f : (v â‡‰ Statement) â†’ Statement) (x y : v â‡‰ Statement) â†’ x â‰…â‚š y â†’ f x â‰…â‚š f y
-- â‰…â‚š-cong {v = []} {[]} f x y xâ‰…y {k} {E} =
--   â‰…â‚›-cong (Î» { (ğ’® s k E) â†’ ğ’® (f s) k E }) (ğ’® x k E) (ğ’® y k E) xâ‰…y
-- â‰…â‚š-cong {v = Î± âˆ· Î±s} {[]} f x y xâ‰…y {k} {E} =
--   let g : (r : Î±) â†’ f (Î» _ â†’ x r) â‰…â‚š f (Î» _ â†’ y r)
--       g r = â‰…â‚š-cong {v = Î±s} {[]} (Î» v â†’ f (Î» _ â†’ v)) _ _ (xâ‰…y {r})
--   in
--     {!g ? {k} {E}!}
-- â‰…â‚š-cong {v = v} {Î² âˆ· Î²s} f x y xâ‰…y {r} =
--   â‰…â‚š-cong {v = v} {Î²s} (Î» c â†’ f c r) _ _ xâ‰…y

postulate ï¼›-assoc : Associative _â‰…â‚š_ _ï¼›_

Î²-if-true : âˆ€ { x y : Statement }
  â†’ (if true then x else y) â‰…â‚š x
Î²-if-true = â†â‡’â‰…â‚› (â†-if-true true-eval)

Î²-if-false : âˆ€ { x y : Statement } â†’ if false then x else y â‰…â‚š y
Î²-if-false = â†â‡’â‰…â‚› (â†-if-false false-eval)

Î·-if : âˆ€ { cond : Expr Bool } { e : Statement } â†’ if cond then e else e â‰…â‚š e
Î·-if {cond}
  with âŠ¢-total {e = cond}
... | (ğ”¹.false , â‡’false) = â†â‡’â‰…â‚› (â†-if-false â‡’false)
... | (ğ”¹.true , â‡’true) = â†â‡’â‰…â‚› (â†-if-true â‡’true)

Î²-while : âˆ€ { eâ‚ : Expr Bool } { eâ‚‚ : Statement }
  â†’ while eâ‚ then eâ‚‚ â‰…â‚š if eâ‚ then (eâ‚‚ ï¼› while eâ‚ then eâ‚‚) else nop
Î²-while = â†â‡’â‰…â‚› â†-while

â‰”-subst : âˆ€ { Î± } { x : Ref Î± } { e : Expr Î± } { f : Expr Î± â†’ Statement }
  â†’ (x â‰” e ï¼› f (â˜… x)) â‰…â‚š (f e)
-- â‰”-subst {Î±} {x} {e} {f} {k} {E}
--   with âŠ¢-total {Î±} {E} {e}
-- ... | v , â‡’v
--     with â‰…â‚›-subst {f = f} (deref {x Env.â†¦ v , E} {Î±} {x} xâ†¦vâˆˆxâ†¦v,E) â‡’v refl
-- ...   | injâ‚ (A , f[â˜…x]â†A , f[e]â†A) =
--         let reduction = â†-seq â—… â†-assignment â‡’v âŸ¨ ? âŸ© â—… â†-nop âŸ¨ ? âŸ© â—… Îµ âŸ¨ ? âŸ© in
--           injâ‚ (A , reduction â—…â—… f[â˜…x]â†A , f[e]â†A)
-- ...   | injâ‚‚ (f[â˜…x]â†Ï‰ , f[e]â†Ï‰) =
--         let reduction = â†-seq â—… â†-assignment â‡’v âŸ¨ ? âŸ© â—… â†-nop âŸ¨ ? âŸ© â—… Îµ âŸ¨ ? âŸ© in
--           injâ‚‚ (â†Ï‰-transáµ‡ reduction f[â˜…x]â†Ï‰ , f[e]â†Ï‰)

decl-elim : âˆ€ { Î± } { f : Statement } â†’ (decl Î± Î» x â†’ f) â‰…â‚š f
decl-elim {Î±} {f} = â‰…â‚›-decl

effects-of (reduce (ğ’® s k E)) â‰ˆ effects-of (ğ’® s stop E) ++ effect-of (k)

nested-while-loop : âˆ€ { s t : Statement }
  â†’ s â‰…â‚š t â†’ while true then s â‰…â‚š while true then (while true then t)
nested-while-loop {s} {t} sâ‰…t {k} {E} =
  â‰ˆR.begin
    effects-of (reduce (ğ’® (while true then s) k E))
  â‰ˆâŸ¨ effects-det (reduce-det _ p) âŸ©
    effects-of p
  â‰ˆâŸ¨ effects-Ï„ âŸ© _
  â‰ˆâŸ¨ effects-Ï„ âŸ© _
  â‰ˆâŸ¨ effects-Ï„ âŸ©
    effects-of (reduce (ğ’® s ((while true then s) then k) E))
  â‰ˆâŸ¨ sâ‰…t âŸ©
    effects-of (reduce (ğ’® t ((while true then s) then k) E))
  â‰ˆâŸ¨ {!nested-while-loop sâ‰…t!} âŸ©
    effects-of (reduce (ğ’® t ((while true then t) then (while true then (while true then t)) then k) E))
  â‰ˆË˜âŸ¨ effects-Ï„ âŸ© _
  â‰ˆË˜âŸ¨ effects-Ï„ âŸ© _
  â‰ˆË˜âŸ¨ effects-Ï„ âŸ© _
  â‰ˆË˜âŸ¨ effects-Ï„ âŸ© _
  â‰ˆË˜âŸ¨ effects-Ï„ âŸ© _
  â‰ˆË˜âŸ¨ effects-Ï„ âŸ©
    effects-of q
  â‰ˆâŸ¨ effects-det (reduce-det q _) âŸ©
    effects-of (reduce (ğ’® (while true then (while true then t)) k E))
  â‰ˆR.âˆ
  where
    p : Reduction _~[_]â†_ (ğ’® (while true then s) k E)
    p = â†-while
      âˆ· â™¯ (â†-if-true true-eval
      âˆ· â™¯ (â†-seq
      âˆ· â™¯ reduce _))
    q : Reduction _~[_]â†_ (ğ’® (while true then (while true then t)) k E)
    q = â†-while
      âˆ· â™¯ (â†-if-true true-eval
      âˆ· â™¯ (â†-seq
      âˆ· â™¯ (â†-while
      âˆ· â™¯ (â†-if-true true-eval
      âˆ· â™¯ (â†-seq âˆ· â™¯ reduce _)))))
    a : effects-of p â‰ˆ effects (ğ’® s ((while true then s) then k) E)
    
-- nested-while-loop {s} {t} sâ‰…t =
--   begin'
--     (while true then s)
--     â‰…âŸ¨ â‰…â‚š-cong {0} (Î» s â†’ while true then s) s t sâ‰…t âŸ©
--     (while true then t)
--     â‰…âŸ¨ â†â‡’â‰…â‚› â†-while âŸ©
--     (if true then (t ï¼› while true then t) else nop)
--     â‰…âŸ¨ Î²-if-true âŸ©
--     (t ï¼› while true then t)
--     â‰…âŸ¨ {!!} âŸ©
--     ((t ï¼› while true then t) ï¼› while true then (while true then t))
--     â‰…âŸ¨ {!!} âŸ©
--     (if true then (t ï¼› while true then t) else nop ï¼› while true then (while true then t))
--     â‰…âŸ¨ {!!} âŸ©
--     (while true then t ï¼› while true then (while true then t))
--     â‰…Ë˜âŸ¨ Î²-if-true âŸ©
--     (if true then (while true then t ï¼› while true then (while true then t)) else nop)
--     â‰…Ë˜âŸ¨ â†â‡’â‰…â‚› â†-while âŸ©
--     (while true then (while true then t))
--   âˆ'

-- Need to ensure s and t don't affect e
nested-while-loop' : âˆ€ { s t : Statement } { e : Expr Bool }
  â†’ s â‰…â‚š t â†’ while e then s â‰…â‚š while e then (while e then t)
